3A)
$$2(b-1)(b^{m-1})(R-r+1)$$

3C)
$$f(x, b, e) := (\sum_{j=1}^{|x|}x_jb^{-j})b^e$$
$$\left\{f(x, b,\ e)\ |\ x\in\{k|\ \|k\| <m ,\ m\in \mathbb{N},\ m> 0\},\ r \leq e \leq R\ \right\}$$
Daraus folgt:
$$ \min f(x, b, e), $$
und:
$$\max f(x, b, e)$$

$$\frac{\delta f}{\delta e} f(x,b,e) = (\sum_{j=1}^{|x|}x_jb^{-j})b^e\ln(b)$$
$$\frac{\delta f}{\delta b} f(x,b,e) =(\sum_{j=1}^{|x|}-jx_jb^{-j-1})\times e\times b^{e-1}$$
$$\frac{\delta f}{\delta x} f(x,b,e) = (\sum_{j=1}^{|x|}b^{-j})b^e$$




$$
\begin{align}

\left(\sum_{j=1}^{m}b^{-j}\right)b^e &= 0 \\
\left(\sum_{j=1}^{m}-jx_jb^{-j-1}\right)\times e\times b^{e-1} &=0\\
\left(\sum_{j=1}^{m}x_jb^{-j}\right)b^e\ln(b)&=0\\
\\
\left(\sum_{j=1}^{m}b^{-j}\right) &= 0 \\
\left(\sum_{j=1}^{m}-jx_jb^{-j-1}\right) \frac{e}{b} &=0\\
\left(\sum_{j=1}^{m}x_jb^{-j}\right)\ln(b)&=0\\
\\
\frac{1}{\sum_{j=1}^{m}x_j} &=0\\
\frac{-m(m+1)e}{2b^2} &= 0 \\
\ln(b) &=0 \\
\\
b &= e^0


\end{align}
$$








$$f'(x,b,e) = (\sum_{j=1}^{|x|}x_jb^{-j})b^e\ln(b)+(\sum_{j=1}^{|x|}-jx_jb^{-j-1})\times e\times b^{e-1}+(\sum_{j=1}^{|x|}b^{-j})b^e$$
$$f'(x,b,e) = b^e((\sum_{j=1}^{|x|}x_jb^{-j})\ln(b)+(\sum_{j=1}^{|x|}-jx_jb^{-j-1}) \frac{e}{b}+(\sum_{j=1}^{|x|}b^{-j}))$$
$$f'(x,b,e) = b^e(\sum_{j=1}^{|x|}x_jb^{-j})(\ln(b)+\frac{-|x|(|x|+1)e}{2b^2}+\frac{1}{\sum_{j=1}^{|x|}x_j})$$
$$f'(x,b,e) = 0 \Rightarrow \sum_{j=1}^{|x|}x_jb^{-j} = 0 \lor \ln(b)+\frac{-|x|(|x|+1)e}{2b^2}+\frac{1}{\sum_{j=1}^{|x|}x_j} = 0$$
Weil nach einer Null verschiedenen zahl gefragt wird muss nun folgende bedingung erf√ºllt werden um 
$$\ln(b)+\frac{-m(m+1)e}{2b^2}+\frac{1}{\sum_{j=1}^{m}x_j} = 0$$
$$$$