
# Theorieaufgabe 1
![[Pasted image 20221115113026.png]]

# Theorieaufgabe 2
Weil
$$
\begin{align}
Ax&=b\\
A\tilde{x}&= b-\tilde{r}
\end{align}
$$
ist:
$$A(x-\tilde{x}) =\tilde{r}$$


um $\kappa(A)^{-1}\frac{\lVert \tilde{r} \rVert}{\lVert b\rVert} \leq \frac{\lVert x-\tilde{x}\rVert}{\lVert x\rVert}$ zu zeigen kann mit etwas einsetzen und umformen:
$$
\begin{align}
&& \kappa(A)^{-1}\frac{\lVert \tilde{r} \rVert}{\lVert b\rVert} &= \frac{\lVert A(x-\tilde{x})\rVert}{\lVert A\rVert \lVert A^{-1}\rVert\lVert Ax\rVert} \\

\Rightarrow&& \kappa(A)^{-1}\frac{\lVert \tilde{r} \rVert}{\lVert b\rVert} &\leq \frac{\lVert x-\tilde{x}\rVert}{\lVert A^{-1}(Ax)\rVert} \\

\Rightarrow && \kappa(A)^{-1}\frac{\lVert \tilde{r} \rVert}{\lVert b\rVert} &\leq \frac{\lVert x-\tilde{x}\rVert}{\lVert x\rVert}
\end{align}
$$

und um $\frac{\lVert x-\tilde{x}\rVert}{\lVert x\rVert} \leq \kappa(A) \frac{\lVert \tilde{r} \rVert}{\lVert b\rVert}$  zu zeigen:
$$
\begin{align}
x-\tilde{x} = A^{-1}\tilde r \ \Leftrightarrow  \ A(x-\tilde{x}) =\tilde{r}\\

&& \lVert x-\tilde x \rVert \lVert b \rVert &= \lVert A^{-1} \tilde r \rVert \lVert Ax \rVert \\

\Rightarrow&& \lVert x-\tilde x \rVert \lVert b \rVert &\leq \lVert A^{-1}\rVert \lVert\tilde r \rVert \lVert A\rVert \lVert x \rVert \\

\Rightarrow&& \lVert x-\tilde x \rVert \lVert b \rVert &\leq \kappa(A) \lVert \tilde{r} \rVert \lVert b\rVert \\

\Rightarrow&& \frac{\lVert x-\tilde{x}\rVert}{\lVert x\rVert} &\leq \kappa(A) \frac{\lVert \tilde{r} \rVert}{\lVert b\rVert} \\
\end{align}
$$
# Theorieaufgabe 3
